\documentclass{article}

\usepackage{fancyhdr}
\usepackage{amsmath}
\usepackage{amsthm}
\usepackage{amssymb}
\usepackage{amsfonts}
\usepackage{extramarks}
\usepackage{derivative}
\usepackage{nicematrix}
\usepackage{tikz}
\usepackage[english]{babel}
\usepackage{physunits}

%
% Basic Document Settings
%
\topmargin=-0.45in
\evensidemargin=0in
\oddsidemargin=0in
\textwidth=6.5in
\textheight=9.0in
\headsep=0.25in

\linespread{1.1}

\pagestyle{fancy}
\rhead{\textbf{\authorName}}
\chead{\textbf{Exercises for \textit{\bookTitle}}}
\cfoot{\thepage}
\lhead{\firstxmark}
\lfoot{\lastxmark}

\renewcommand\headrulewidth{0.4pt}
\renewcommand\footrulewidth{0.4pt}

\setlength\parindent{0pt}

%
% Create Exercise Sections
%
\newcommand{\enterExerciseHeader}[1]{
    \nobreak\extramarks{}{Exercise \arabic{#1} continued on next page\ldots}\nobreak{}
    \nobreak\extramarks{Exercise \arabic{#1} (continued)}{Exercise \arabic{#1} continued on next page\ldots}\nobreak{}
}

\newcommand{\exitExerciseHeader}[1]{
    \nobreak\extramarks{Exercise \arabic{#1} (continued)}{Exercise \arabic{#1} continued on next page\ldots}\nobreak{}
    \stepcounter{#1}
    \nobreak\extramarks{Exercise \arabic{#1}}{}\nobreak{}
}

\setcounter{secnumdepth}{0}
\newcounter{partCounter}
\newcounter{exerciseCounter}
\setcounter{exerciseCounter}{1}
\nobreak\extramarks{Exercise \arabic{exerciseCounter}}{}\nobreak{}

\newenvironment{exercise}[1][-1]{
    \ifnum#1>0
        \setcounter{exerciseCounter}{#1}
    \fi
    \section{Exercise \arabic{exerciseCounter}}
    \setcounter{partCounter}{1}
    \enterExerciseHeader{exerciseCounter}
}{
    \exitExerciseHeader{exerciseCounter}
}

\newcommand{\Z}{\mathbb{Z}}
\newcommand{\R}{\mathbb{R}}

\newcommand{\bookTitle}{Special Relativity}
\newcommand{\bookAuthor}{Nick Woodhouse}
\newcommand{\authorName}{Max Besley}

%
% Title Page
%
\title{
    \vspace{2in}
    \textmd{\textbf{\bookTitle:\ Exercises}}\\
    \vspace{0.1in}\large{\textbf{Textbook by \bookAuthor}}
    \vspace{3in}
}

\author{\textbf{\authorName}}
\date{}

\newcommand{\vect}[1]{\ensuremath{\mathbf{#1}}}
\newcommand{\norm}[1]{\left\lVert#1\right\rVert}
\renewcommand\qedsymbol{$\blacksquare$}

\renewcommand{\part}[1]{\textbf{\large Part \Alph{partCounter}}\stepcounter{partCounter}\\}

% Alias for the Solution section header
\newcommand{\solution}{\textbf{\large Solution}}

\begin{document}

\maketitle

\pagebreak

\section{\underline{\Large{Chapter 1}}} \vspace{5mm}

\begin{exercise}[1]
    Showing associativity is omitted. \\

    \textbf{Identity:} \\
    Set $H=I_3$ and $C=\vect{0}$ and this isometry is the identity. \\

    \textbf{Closure:} \\
    Assume $\phi(\boldsymbol{x})=H_1\vect{x}+C_1$ and $\psi(\vect{x})=H_2\vect{x}+C_2$ are isometries of $\mathbb{E}$. \\
    We have,
    \begin{equation} \tag{*}
    \begin{split}
        (\psi\circ\phi)(\vect{x}) & = \psi(\phi(\vect{x})) \\
                                  & = \psi(H_1\vect{x}+C_1) \\
                                  & = H_2(H_1\vect{x}+C_1)+C_2 \\
                                  & = H_2H_1\vect{x}+(H_2C_1+C_2)
    \end{split}
    \end{equation}
    and so the map $\psi\circ\phi$ is also an isometry of $\mathbb{E}$. \\

    \textbf{Inverses:} \\
    Let $\psi(\vect{x})=H\vect{x}+C$ be an isometry of $\mathbb{E}$. \\
    The inverse isometry map is $\psi^{-1}(\vect{x})=H^{-1}\vect{x}-H^{-1}C$.
    In particular it's easy to check that $(\psi^{-1}\circ\psi)(\vect{x})=
    \vect{x}=(\psi\circ\psi^{-1})(\vect{x})$ for any $\vect{x}\in\mathbb{E}$. \\

    Hence the isometries of Euclidean space form a group. \\

    We now show that the proper (orientation-preserving) isometries form a subgroup. \\

    The identity map is a proper isometry since $\text{det}(I_3)=0$.
    The composition of two proper isometries is a proper isometry because we will have
    $\text{det}(H_2H_1)=\text{det}(H_2)\text{det}(H_1)=1\cdot1=1$ in equation (*).
    Lastly, if $\psi(\vect{x})=H\vect{x}+C$ is a proper isometry we have $\text{det}(H^{-1})=\text{det}(H)^{-1}=1^{-1}=1$ and so the inverse map $\psi^{-1}$ is also
    a proper isometry. Thus the proper isometries of $\mathbb{E}$ form a subgroup.
\end{exercise}

\NiceMatrixOptions
{
    custom-line ={command= H, tikz= dashed, width= 1mm}, % horizontal, dashed
    custom-line = {letter= I, tikz= dashed, width= 1mm}, % vertical, dashed
}

\begin{exercise}[2]
    (i)
    We have
    \begin{gather*}
    t = t^\prime + c_0 \\
    x=v_1 t^\prime + H_{11}x^\prime + H_{12}y^\prime + H_{13}z^\prime + c_1 \\
    y=v_2 t^\prime + H_{21}x^\prime + H_{22}y^\prime + H_{23}z^\prime + c_2 \\
    z=v_3 t^\prime + H_{31}x^\prime + H_{32}y^\prime + H_{33}z^\prime + c_3
    \end{gather*}
    and by the first equation $\odv{t^\prime}{t}=1$. Using the chain rule,
    \begin{align*}
    \odv{x}{t}=\odv{x}{t^\prime}\odv{t^\prime}{t}= v_1 \cdot 1 = v_1
    \end{align*}
    and likewise $\odv{y}{t}=v_2$ and $\odv{z}{t}=v_3$. \\\\
    Thus we have $\vect{v}=\left(\odv{x}{t},\odv{y}{t},\odv{z}{t}\right)=\left(v_1,v_2,v_3\right)$
    where $\vect{v}$ is the velocity of $R^\prime$ relative to the frame of
    reference $R$. \\

    (ii)
    Suppose we have a second Galilean transformation \\
    \begin{align*}
        \begin{bmatrix} t^\prime \\ x^\prime \\ y^\prime \\ z^\prime \end{bmatrix}
        =
        \begin{bNiceMatrix}
            1 & 0 & 0 & 0 \\
            w_1 & K_{11} & K_{12} & K_{13} \\
            w_2 & K_{21} & K_{22} & K_{23} \\
            w_3 & K_{31} & K_{32} & K_{33}
        \end{bNiceMatrix}
        \begin{bmatrix} t^{\prime\prime} \\ x^{\prime\prime} \\ y^{\prime\prime} \\ z^{\prime\prime} \end{bmatrix}
        + \begin{bmatrix} d_0 \\ d_1 \\ d_2 \\ d_3 \end{bmatrix}
    \end{align*}

    Composing with the first Galilean transformation gives
    \begin{align*}
        \begin{bmatrix} t \\ x \\ y \\ z \end{bmatrix} &=
        \begin{bNiceMatrix}
            1 & 0 & 0 & 0 \\
            v_1 & H_{11} & H_{12} & H_{13} \\
            v_2 & H_{21} & H_{22} & H_{23} \\
            v_3 & H_{31} & H_{32} & H_{33}
        \end{bNiceMatrix}
        \left(
        \begin{bNiceMatrix}
            1 & 0 & 0 & 0 \\
            w_1 & K_{11} & K_{12} & K_{13} \\
            w_2 & K_{21} & K_{22} & K_{23} \\
            w_3 & K_{31} & K_{32} & K_{33}
        \end{bNiceMatrix}
        \begin{bmatrix} t^{\prime\prime} \\ x^{\prime\prime} \\ y^{\prime\prime}
        \\ z^{\prime\prime} \end{bmatrix}
        + \begin{bmatrix} d_0 \\ d_1 \\ d_2 \\ d_3 \end{bmatrix}
        \right)
        + \begin{bmatrix} c_0 \\ c_1 \\ c_2 \\ c_3 \end{bmatrix} \\[1em]
        &=
        \begin{bNiceArray}{cIccc}[margin]
            1 & 0 & 0 & 0 \\ \H
            \Block{3-1}{\vect{v}+H\vect{w}} & \Block[c]{3-3}<\large>{HK} \\
            & & & \\
            & & &
        \end{bNiceArray}
        \begin{bmatrix} t^{\prime\prime} \\ x^{\prime\prime} \\ y^{\prime\prime}
        \\ z^{\prime\prime} \end{bmatrix} +
        \begin{bNiceMatrix} d_0 \\ \Block{*-1}{d_0\vect{v}+H\vect{d}} \end{bNiceMatrix}
        + \begin{bmatrix} c_0 \\ c_1 \\ c_2 \\ c_3 \end{bmatrix}
    \end{align*}
    which again is a Galilean transformation as $HK \in SO(3)$.
    Here $\vect{v}=\begin{bmatrix} v_1 \\ v_2 \\ v_3 \end{bmatrix}$,
    $\vect{w}=\begin{bmatrix} w_1 \\ w_2 \\ w_3 \end{bmatrix}$
    and $\vect{d}=\begin{bmatrix} d_1 \\ d_2 \\ d_3 \end{bmatrix}$. \\[0.5em]

    The above vector $\vect{v}+H\vect{w}$ is consistent with the classical velocity addition
    law. Recall that the vector $\vect{w}$ comes from the inertial frame $R^\prime$, and
    so the orthogonal matrix $H$ is applied in order to translate from the coordinates
    of $R^\prime$ into the coordinates of the inertial frame $R$. \\

    The inverse of a general Galilean transformation is \\
    \begin{equation*}
        \begin{bmatrix} t^\prime \\ x^\prime \\ y^\prime \\ z^\prime \end{bmatrix}
        =
        \begin{bNiceArray}{cIccc}[margin]
            1 & 0 & 0 & 0 \\ \H
            \Block{3-1}{H^{-1}(\vect{-v})} & \Block[c]{3-3}<\large>{H^{-1}} \\
            & & & \\
            & & &
        \end{bNiceArray}
        \begin{bmatrix} t \\ x \\ y \\ z \end{bmatrix}
        + \begin{bNiceMatrix} -c_0 \\ \Block{*-1}{H^{-1}(c_0\vect{v}-\vect{c})} \end{bNiceMatrix}
    \end{equation*} \\
    which is a Galilean transformation as $H^{-1} \in SO(3)$. \\

    (iii) (A) \\
    A Galilean transformation performs the mapping $t_i \mapsto t^{\prime}_i + c_0$
    (where $i\in\{1,2\}$) on the two time coordinates. So the time separation between
    the two events in the new frame $R^\prime$ is $t^{\prime}_2+c_0-(t^{\prime}_1+c_0)
    =t^{\prime}_2-t^{\prime}_2=t_2-t_1$, using the fact that $t=t^\prime$ in Galilean relativity. \\

    (iii) (B) \\
    Assume that $t_1=t_2$. \\
    Observe that a Galilean transformation maps the coordinates $(t_1,x_1,y_1,z_1)$
    and $(t_2,x_2,y_2,z_2)$ to the new coordinates:
    \begin{align*}
        \begin{bNiceMatrix} t_1+c_0 \\ \Block{*-1}{\vect{v}t_1+H\vect{r_1}+\vect{c}} \end{bNiceMatrix}
        \hspace{1em} \text{and} \hspace{1em}
        \begin{bNiceMatrix} t_2+c_0 \\ \Block{*-1}{\vect{v}t_2+H\vect{r_2}+\vect{c}} \end{bNiceMatrix}
    \end{align*}
    where $\vect{r_i}=\begin{bmatrix} x_i \\ y_i \\ z_i \end{bmatrix}$
    and $\vect{c}=\begin{bmatrix} c_1 \\ c_2 \\ c_3 \end{bmatrix}$. \\[1em]
    Now we compute
    \begin{align*}
        \norm{\begin{bmatrix} x_2^\prime \\ y_2^\prime  \\ z_2^\prime  \end{bmatrix}-
        \begin{bmatrix} x_1^\prime \\ y_1^\prime  \\ z_1^\prime  \end{bmatrix}}
        &= \norm{\vect{v}t_2+H\vect{r_2}+\vect{c}-(\vect{v}t_1+H\vect{r_1}+\vect{c})} \\
        &= \norm{(t_2-t_1)\vect{v}+H\vect{r_2}-H\vect{r_1}} \\
        &= \norm{H\vect{r_2}-H\vect{r_1}} \\
        &= \norm{\vect{r_2}-\vect{r_1}} \\
        &= \sqrt{(x_2-x_1)^2+(y_2-y_1)^2+(z_2-z_1)^2}
    \end{align*}
    and so the distance between the two events is preserved. \\
    If the two events are not simultaneous then one of the frames may have
    moved through space during the time interval $t_2-t_1$, thus increasing or
    decreasing the measured spatial distance between the events. \\

    Here I skip the last part. Perhaps I will do it later.
\end{exercise}

\pagebreak

\section{\underline{\Large{Chapter 2}}} \vspace{5mm}

\begin{exercise}[1]
    (1) \\
    \begin{equation*}
       \begin{split}
        \text{div}(\textbf{\textit{E}}^\prime)&=\text{div }[\text{cos}(\alpha)\textbf{\textit{E}}-\text{sin}(\alpha)c\textbf{\textit{B}}] \\
        &=\text{cos}(\alpha)\text{div}(\textbf{\textit{E}})-\text{sin}(\alpha)c\ \text{div}(\textbf{\textit{B}}) \\
        &=0+0=0
        \end{split}
    \end{equation*}

    (2) \\
    \begin{equation*}
       \begin{split}
        \text{div}(\textbf{\textit{B}}^\prime)&=\text{div }[c^{-1}\text{sin}(\alpha)\textbf{\textit{E}}+\text{cos}(\alpha)\textbf{\textit{B}}] \\
        &=c^{-1}\text{sin}(\alpha)\text{div}(\textbf{\textit{E}})+\text{cos}(\alpha)\text{div}(\textbf{\textit{B}}) \\
         &=0+0=0
        \end{split}
    \end{equation*}

    (3) \\
    \begin{equation*}
       \begin{split}
        \text{curl}(\textbf{\textit{B}}^\prime)&=c^{-1}\text{sin}(\alpha)\text{curl}(\textbf{\textit{E}})+\text{cos}(\alpha)\text{curl}(\textbf{\textit{B}}) \\
        &=c^{-1}\text{sin}(\alpha)\left(-\pdv{\textbf{\textit{B}}}{t}\right)+\text{cos}(\alpha)\frac{1}{c^2}\pdv{\textbf{\textit{E}}}{t} \\
        &=\frac{1}{c^2}\text{cos}(\alpha)\pdv{\textbf{\textit{E}}}{t}-c^{-1}\text{sin}(\alpha)\pdv{\textbf{\textit{B}}}{t} \\
        &=\frac{1}{c^2}\left(\text{cos}(\alpha)\pdv{\textbf{\textit{E}}}{t}-\text{sin}(\alpha)\pdv{\left(c\textbf{\textit{B}}\right)}{t}\right) \\
        &=\frac{1}{c^2}\pdv{\textbf{\textit{E}}^\prime}{t}
        \end{split}
    \end{equation*}

    (4) \\
    \begin{equation*}
       \begin{split}
        \text{curl}(\textbf{\textit{E}}^\prime)&=\text{cos}(\alpha)\text{curl}(\textbf{\textit{E}})-\text{sin}(\alpha)c\ \text{curl}(\textbf{\textit{B}}) \\
        &=\text{cos}(\alpha)\left(-\pdv{\textbf{\textit{B}}}{t}\right)-\text{sin}(\alpha)c\ \frac{1}{c^2}\pdv{\textbf{\textit{E}}}{t} \\
        &=-\left(c^{-1}\text{sin}(\alpha)\pdv{\textbf{\textit{E}}}{t}+\text{cos}(\alpha)\pdv{\textbf{\textit{B}}}{t}\right) \\
        &=-\pdv{\textbf{\textit{B}}^\prime}{t}
        \end{split}
    \end{equation*}
\end{exercise}

\begin{exercise}[2]
    Assume $x^2+y^2<a^2$. \\
    Using an explicit formula for the curl operator we have \\
    \begin{equation*}
       \begin{split}
        \nabla\times\textbf{\textit{B}}&=\nabla\times\left(\frac{I\mu_0(-y\mathbf{\hat{i}}+x\mathbf{\hat{j}})}{2\pi a^2}\right) \\
        &=\frac{I\mu_0}{2\pi a^2}\ \nabla\times\left(-y\mathbf{\hat{i}}+x\mathbf{\hat{j}}\right) \\
        &=\frac{I\mu_0}{2\pi a^2}\ 2\mathbf{\hat{k}} \\
        &=\frac{I\mu_0}{\pi a^2}\mathbf{\hat{k}}
        \end{split}
    \end{equation*}
    Now assuming $x^2+y^2 \geq a^2$ we have
    \begin{equation*}
       \begin{split}
        \nabla\times\textbf{\textit{B}}&=\nabla\times\left(\frac{I\mu_0(-y\mathbf{\hat{i}}+x\mathbf{\hat{j}})}{2\pi (x^2+y^2)}\right) \\
        &=\frac{I\mu_0}{2\pi}\ \nabla\times\left(\frac{-y\mathbf{\hat{i}}+x\mathbf{\hat{j}}}{x^2+y^2}\right) \\
        &=\frac{I\mu_0}{2\pi a^2}\left(\frac{-x^2+y^2}{(x^2+y^2)^2}-\frac{-x^2+y^2}{(x^2+y^2)^2}\right)\mathbf{\hat{k}} \\
        &=\vect{0}
        \end{split}
    \end{equation*}
    Completing the exercise. \\
    See https://pressbooks.online.ucf.edu/osuniversityphysics2/chapter/amperes-law/ for another
    derivation of the magnetic field generated by an electric current in a straight wire.
\end{exercise}

\pagebreak

\section{\underline{\Large{Chapter 4}}} \vspace{5mm}

\begin{exercise}[1]
    (i) \\
    Skipped. This problem is very interesting, but I don't understand
    how to solve it using the chain rule. It's worth coming back to. \\

    (ii) \\
    Assume that $u \ll c$ and the event $\textit{E}$ has coordinates $t^\prime=0$, $x^\prime=-D$
    according to the observer $\mathcal{O}^\prime$. \\
    The Lorentz transformation gives us the relations,
    \begin{gather*}
        t=\gamma\left(t^\prime+\frac{u}{c^2}x^\prime\right) \\
        x=\gamma\left(ut^\prime+x^\prime\right)
    \end{gather*}
    and so $t=\gamma\left(-\frac{u}{c^2}D\right)$ and $x=-\gamma D$. \\
    Because $u \ll c$ the Lorentz factor $\gamma$ is very close to one, and so
    we conclude that $t=-\frac{u}{c^2}D$, $x=-D$. \\\\
    Note that in this example the first observer $\mathcal{O}$ is moving
    in the negative $x^\prime$-direction with speed $u>0$. \\

    (iii) \\
    Denote the event occurring at Andromeda by $\textit{B}$ and denote the woman and the man's
    reference frames by $\mathcal{O}$ and $\mathcal{O}^\prime$, respectively. \\
    According to the woman $t_B=0$ and $x_B=D=2.2\times10^6 \ \ly$. \\
    From the Lorentz transformation between $\mathcal{O}$ and $\mathcal{O}^\prime$ we have
    $t_B^\prime=\gamma\left(t_B-\frac{u}{c^2}x_B\right)$. Thus $t_B^\prime=-\gamma\frac{uD}{c^2}$. \\
    Since the relative speed of the man is so small, the Lorentz factor $\gamma$ is very
    close to one and can be ignored. \\
    We compute,
    \begin{equation*}
        -t_B^\prime=\frac{uD}{c^2}=\frac{(2.2352\mps)(2.2\cdot10^6\times3\cdot10^8\mps)}
        {(3.8\cdot10^8\mps)^2}\ \text{years}=0.01639\ \text{years}=6\ \text{days}
    \end{equation*}
    And so the man might reply by saying: "No, this already happened six days ago."
\end{exercise}

\begin{exercise}[2]
    ($\implies$) \\
    Assume that $L=\gamma\begin{bmatrix} 1 & \beta \\ \beta & 1 \end{bmatrix}$. \\
    The top left entry $\gamma$ is positive and $\text{det }L=\gamma^2(1-\beta^2)>0$
    because $-c<u<c$. \\
    Thirdly,
    \begin{align*}
        L^T\begin{bmatrix} 1 & 0 \\ 0 & -1 \end{bmatrix}L
        &=\gamma^2\begin{bmatrix} 1 & \beta \\ \beta & 1 \end{bmatrix}\begin{bmatrix} 1 & 0 \\ 0 & -1 \end{bmatrix}\begin{bmatrix} 1 & \beta \\ \beta & 1 \end{bmatrix} \\
        &=\gamma^2\begin{bmatrix} 1-\beta^2 & 0 \\ 0 & \beta^2-1 \end{bmatrix} \\
        &=\begin{bmatrix} 1 & 0 \\ 0 & -1 \end{bmatrix}
    \end{align*}

    ($\impliedby$) \\
    Let $L=\begin{bmatrix} p & q \\ r & s \end{bmatrix}$ where $p,q,r,s\in\R$. \\\\
    From (i) and (ii) we have $p>0$ and $ps-qr>0$. \\
    From (iii) we deduce that $pq=rs$, $s^2-q^2=1$ and $p^2-r^2=1$. \\\\
    The equation $s^2-q^2=1$ implies that $s\neq0$ which allows us to divide by $s$. \\
    Setting $\beta=\frac{u}{c}=\frac{q}{s}=\frac{r}{p}$ we have,
    \begin{align*}
        p^2-\left(\frac{pq}{s}\right)^2=1
        &\implies p^2\left(1-\frac{q^2}{s^2}\right)=1 \\
        &\implies p=\gamma
    \end{align*}
    and likewise
    \begin{align*}
        s^2-\left(\frac{rs}{p}\right)^2=1
        &\implies s=\gamma
    \end{align*}

    Then we easily see that
    \begin{align*}
        q=\frac{r}{p}s=\beta\gamma
        &\quad\text{and}\quad r=\frac{q}{s}p=\beta\gamma
    \end{align*}
    Thus the matrix L has the form of a Lorentz transformation. \\

    We also want to show that $\lvert u \rvert < c$. Using (ii),
    \begin{align*}
        0 < \text{det }L
        &\iff 0 < \gamma^2-\beta^2\gamma^2 \\
        &\iff \beta^2 < 1 \\
        &\iff -1 < \beta < 1 \\
        &\iff -c < u < c
    \end{align*}
    This means that the relative speed of the two observers is bounded by the constant
    $c>0$ if and only if the Lorentz transformation satisfies $\text{det }L>0$. \\

    Lastly, the rapidity $\phi$ of the Lorentz transformation can be expressed as
    \begin{align*}
        2\cdot\text{cosh }\phi&=e^\phi+e^{-\phi} \\
        &=k+k^{-1} \\
        &=2\gamma \\
        &=\text{trace }L
    \end{align*}
    where the Bondi k-factor equals the exponential of the rapidity.
\end{exercise}

\begin{exercise}[3]
    Skipped. This is the classic "pole and barn" paradox.
\end{exercise}

\begin{exercise}[4]
    Assume the two light sources are moving to the right with speed $u>0$. \\

    Notice that
    \begin{itemize}
    \item Because the apparatus is now moving the two light sources are a distance $\gamma^{-1}D$ apart, due to length contraction.
    \item Because of the relativity of simultaneity the light source to the left emits a photon
    $\gamma\frac{uD}{c^2}$ seconds before the light source to the right emits its corresponding photon.
    \item The light source on the right-hand side moves a distance $u\cdot\gamma\frac{uD}{c^2}$
    in the time between the two photons being emitted.
    \end{itemize}

    Reasoning from a diagram and these observations, the spatial separation between
    the photons in the frame in which the light sources are moving is:
    \begin{equation*}
        \gamma^{-1}D+u\cdot\gamma\frac{uD}{c^2}-c\cdot\gamma\frac{uD}{c^2}
    \end{equation*}

    This becomes
    \begin{align*}
        \gamma^{-1}D+u\cdot\gamma\frac{uD}{c^2}-c\cdot\gamma\frac{uD}{c^2}&=
        \gamma D\left(\gamma^{-2}+\beta^2-\beta\right) \\
        &=\gamma D\left(1-\beta\right) \\
        &=D\sqrt{\frac{(1-\beta)^2}{1-\beta^2}} \\
        &=D\sqrt{\frac{(1-\beta)^2}{(1-\beta)(1+\beta)}} \\
        &=D\sqrt{\frac{1-\beta}{1+\beta}} \\
        &=D\sqrt{\frac{c-u}{c+u}} \\
    \end{align*}
    as required. \\\\
    If the light sources were moving to the left with speed $u>0$,
    the argument would be similar and would give a final answer
    of $D\sqrt{\frac{c+u}{c-u}}$.
\end{exercise}

\end{document}

